examples/proofs/UnionFind/math/UnionFind04Compress.v
@@ -1,38 +1,43 @@
-Set Implicit Arguments.
-From TLC Require Import LibTactics LibLogic LibProd LibContainer LibSet
-     LibRelation LibPer.
-Local Notation path := rtclosure.
-From iris_time.union_find.math Require Import TLCBuffer UnionFind01Data.
+From osiris Require Import osiris.
+From stdpp Require Import relations propset.
+Require Import UnionFind01Data.
 
 (* -------------------------------------------------------------------------- *)
 
+(* We consider what happens when one performs one step of path compression:
+   given an edge from [x] to [y] and a path from [y] to [z], we replace the
+   edge from [x] to [y] with an edge from [x] to [z]. *)
+
+(* This is a scoped-down port: it covers only what UnionFind.v's [Mem_compress]
+   needs (the definition of [compress] and the lemmas that don't depend on the
+   [F x y]/[path F y z] hypotheses). The rest of the original file
+   (is_dsf_compress, compress_preserves_is_repr[_direct['], _is_equiv,
+   _dsf_per, _descendants_of_roots, _paths_*, the "weak" variants,
+   compress_R_compress_agree, compress_compress) characterizes how [compress]
+   interacts with a *specific* edge [x -> y] and the path beyond it; that's
+   needed for [find_spec_inductive]'s iterated-compression argument
+   (UnionFind05IteratedCompression.v), which belongs to the deferred
+   function-specification phase, not the Mem/Inv layer. *)
+
 Section PathCompression.
 
-(* We now consider what happens when one performs one step of path compression.
-   We assume that there is an edge from [x] to [y] and a path from [y] to [z].
-   We do not require [z] to be a root, as this is in principle unnecessary. We
-   replace the edge of [x] to [y] with an edge from [x] to [z]. *)
-
 Variable V : Type.
-Variable F : binary V.
+Variable EqV : EqDecision V.
+Variable CountableV : Countable V.
+Variable F : relation V.
 Variable x z : V.
 
-(* Path compression is performed as follows. We first corestrict [F] to [x],
-   then take the union with the singleton [per_single x z]. *)
+(* Path compression is performed as follows: every edge out of [x] is
+   removed, and a new edge from [x] to [z] is installed. *)
 
-Definition compress : binary V :=
+Definition compress : relation V :=
   fun a b => (F a b /\ a <> x) \/ (a = x /\ b = z).
-
-Ltac by_cases_on_compress :=
-  unfold compress in *; branches; unpack; subst.
 
 (* We have a new edge from [x] to [z]. *)
 
 Lemma compress_x_z:
   compress x z.
-Proof using.
-  unfold compress. eauto.
-Qed.
+Proof. right. split; reflexivity. Qed.
 
 (* Every existing edge whose source is not [x] is preserved. *)
 
@@ -41,353 +46,31 @@ Lemma compress_preserves_other_edges:
   F v w ->
   v <> x ->
   compress v w.
-Proof using.
-  unfold compress. eauto.
-Qed.
+Proof. intros v w HF Hneq. left. split; assumption. Qed.
 
-Lemma compress_preserves_other_edges_converse:
-  forall v w,
-  compress v w ->
-  v <> x ->
-  F v w.
-Proof using.
-  unfold compress. intros. branches; unpack; subst. eauto. tauto.
-Qed.
+(* Every root other than [x] remains a root. *)
 
 Lemma compress_preserves_roots_other_than_x:
   forall r,
   r <> x ->
-  is_root F r ->
-  is_root compress r.
-Proof using.
-  unfold is_root, not. intros. by_cases_on_compress; eauto.
+  is_root V F r ->
+  is_root V compress r.
+Proof.
+  intros r Hneq Hroot w Hcomp.
+  destruct Hcomp as [[HF _] | [Heq _]].
+  - eapply Hroot; eauto.
+  - apply Hneq. exact Heq.
 Qed.
 
 Lemma compress_preserves_roots_converse:
   forall r,
-  is_root compress r ->
-  is_root F r.
-Proof using.
-  unfold is_root, compress. intros r hr v ?.
-  tests : (r = x); eapply hr; eauto.
-Qed.
-
-(* -------------------------------------------------------------------------- *)
-
-(* The following hypotheses are introduced only now, as they are not needed
-   by the above lemmas. *)
-
-Variable y : V.
-Hypothesis x_edge_y:  F x y.
-
-(* [is_root] is preserved. *)
-
-Lemma compress_preserves_roots:
-  forall r,
-  is_root F r ->
-  is_root compress r.
-Proof using x_edge_y.
-  unfold is_root, not. intros. by_cases_on_compress; eauto.
-Qed.
-
-(* -------------------------------------------------------------------------- *)
-
-(* The following hypotheses are introduced only now, as they are not needed
-   by the above lemmas. *)
-
-Variable D : set V.
-Hypothesis is_dsf_F:  is_dsf D F.
-Hypothesis y_path_z:  path F y z.
-
-(* Every path out of [y] is preserved. *)
-
-Lemma compress_preserves_paths_out_of_y:
-  forall v w,
-  path F v w ->
-  path F y v ->
-  path compress v w.
-Proof using x_edge_y is_dsf_F y_path_z.
-  induction 1 using rtclosure_ind_l; [| rename x0 into v, z0 into w ]; intros.
-    { eauto with rtclosure. }
-    { (* Because there is a path from [y] to [v], [v] cannot be [x],
-         as there would otherwise be a cycle. *)
-      assert (x <> v).
-        { applys* paths_have_distinct_endpoints.
-          applys* tclosure_of_rtclosure_r y. }
-      (* Thus, we can follow the old edge out of [v]: it is preserved. *)
-      eauto using rtclosure_l, rtclosure_r, compress_preserves_other_edges. }
-Qed.
-
-(* Every path out of [z] is preserved. *)
-
-Lemma compress_preserves_paths_out_of_z:
-  forall v w,
-  path F v w ->
-  path F z v ->
-  path compress v w.
-Proof using x_edge_y is_dsf_F y_path_z.
-  eauto using compress_preserves_paths_out_of_y, rtclosure_trans_explicit.
-Qed.
-
-(* Every path to a root is preserved. *)
-
-Lemma compress_preserves_paths_to_roots:
-  forall v r,
-  path F v r ->
-  is_root F r ->
-  path compress v r.
-Proof using x_edge_y is_dsf_F y_path_z.
-  induction 1 as [| w v r ] using rtclosure_ind_l; intros.
-  eauto with rtclosure.
-  destruct (classic (x = v)).
-    { subst v.
-      (* Assume the path begins at [x]. Then, [r] must be the representative
-         of [x]. *)
-      assert (is_repr F x r).
-        { eauto with is_repr. }
-      (* Because [x] and [z] are equivalent, [r] is also the representative
-         of [z]. *)
-      assert (is_repr F z r).
-        { eauto with is_repr. }
-      (* Hence, there is a path of [z] to [r], and by the previous lemma,
-         this path is preserved. Thus, after compression, one can go from
-         [x] to [r] by taking the new edge from [x] to [z] and from there
-         by following the same path as before. *)
-        eapply rtclosure_l.
-        eauto using compress_x_z.
-        eauto using compress_preserves_paths_out_of_z, is_repr_path with rtclosure. }
-    (* If the path does not begin at [x], then its first edge is preserved.
-       Just follow it and continue. *)
-    { eapply rtclosure_l; eauto using compress_preserves_other_edges. }
-Qed.
-
-(* [is_repr] is preserved. *)
-
-Lemma compress_preserves_is_repr_direct:
-  forall x r,
-  is_repr F x r ->
-  is_repr compress x r.
-Proof using x_edge_y is_dsf_F y_path_z.
-  unfold is_repr. intros. unpack.
-  eauto using compress_preserves_paths_to_roots, compress_preserves_roots.
-Qed.
-
-Lemma compress_preserves_is_repr_direct':
-  forall x r,
-  is_root F z ->
-  is_repr F x r ->
-  is_repr compress x r.
-Proof using x_edge_y is_dsf_F y_path_z.
-  Local Hint Unfold is_repr : core.
-  intros x' r' Rz [Pr' Rr']. split.
-  { induction Pr' as [r'|y' x' z'] using rtclosure_ind_l.
-    { now constructor. }
-    { tests E: (x' = x).
-      { asserts: (y' = y). applys* is_dsf_functional. subst.
-        asserts: (z' = z). applys* functional_is_repr y. subst.
-        unfold compress. applys* rtclosure_once. }
-      { unfold compress. applys* rtclosure_l. } } }
-  { applys~ compress_preserves_roots. }
-Qed.
-
-(* The structure of a disjoint set forest is preserved. *)
-
-Lemma is_dsf_compress:
-  is_dsf D compress.
-Proof using x_edge_y is_dsf_F y_path_z.
-  splits.
-  (* [confined] *)
-  { unfold confined. intros. by_cases_on_compress.
-      eauto 6 with confined.
-      split.
-        (* x \in D *) eauto with confined.
-        (* z \in D *) eauto with sticky confined. }
-  (* [functional] *)
-  { unfold functional. intros. repeat by_cases_on_compress;
-      try solve [ exploit_functional F; eauto | eauto | false ]. }
-  (* [defined]. *)
-  { intro v.
-    forwards [ r ? ]: is_dsf_defined_is_repr v. eauto.
-    eauto using compress_preserves_is_repr_direct. }
-Qed.
-
-Local Hint Resolve is_dsf_compress : functional.
-
-(* [is_repr] is preserved (both ways). *)
-
-Lemma compress_preserves_is_repr:
-  is_repr F =
-  is_repr compress.
-Proof using x_edge_y is_dsf_F y_path_z.
-  eapply eq_of_incl_defined_functional.
-    unfold rel_incl. eauto using compress_preserves_is_repr_direct.
-    eauto using is_dsf_defined_is_repr.
-    eauto with functional.
-Qed.
-
-(* [is_equiv] is preserved. *)
-
-Lemma compress_preserves_is_equiv:
-  is_equiv F =
-  is_equiv compress.
-Proof using x_edge_y is_dsf_F y_path_z.
-  unfold is_equiv. rewrite compress_preserves_is_repr. reflexivity.
-Qed.
-
-(* [dsf_per] is preserved. *)
-
-Lemma compress_preserves_dsf_per:
-  dsf_per D F =
-  dsf_per D compress.
-Proof using x_edge_y is_dsf_F y_path_z.
-  unfold dsf_per. rewrite compress_preserves_is_equiv. reflexivity.
-Qed.
-
-(* The descendants of every root are preserved. *)
-
-Lemma compress_preserves_descendants_of_roots:
-  forall r,
-  is_root compress r -> (* or: [is_root F r] *)
-  descendants compress r = descendants F r.
-Proof using x_edge_y is_dsf_F y_path_z.
-  intros. eapply set_ext. intros v.
-  assert (is_root F r). eauto using compress_preserves_roots_converse.
-  repeat rewrite descendant_of_a_root by eauto using compress_preserves_roots.
-  rewrite compress_preserves_is_repr.
-  tauto.
-Qed.
-
-(* No new paths are created. *)
-
-Lemma compress_preserves_paths_converse:
-  forall u w,
-  path compress u w ->
-  path F u w.
-Proof using x_edge_y y_path_z. (* note: is_dsf_F not needed *)
-  induction 1 as [| v u w ] using rtclosure_ind_l; intros; subst.
-  { eauto with rtclosure. }
-  { by_cases_on_compress.
-    (* Case [u <> x]. This edge cannot be new. *)
-    { eauto with rtclosure. }
-    (* Case [u = x]. There is a path from [x] to [z] in [F], followed
-       with a path from [z] to [w], by the induction hypothesis. *)
-    { eauto using rtclosure_trans_explicit with rtclosure. }}
-Qed.
-
-(* The ancestors of [y] are not affected. *)
-
-Lemma ancestors_compress:
-  ancestors compress y \c ancestors F y.
-  (* one could prove an equality, if needed *)
-Proof using x_edge_y y_path_z.
-  unfold ancestors. intros. eapply incl_prove. intros. rew_set in *.
-  eauto using compress_preserves_paths_converse.
+  is_root V compress r ->
+  is_root V F r.
+Proof.
+  intros r Hroot w HF.
+  destruct (decide (r = x)) as [-> | Hneq].
+  - eapply Hroot. right. split; reflexivity.
+  - eapply Hroot. left. split; [exact HF | exact Hneq].
 Qed.
 
 End PathCompression.
-
-Global Hint Resolve compress_preserves_roots compress_preserves_roots_converse : is_root.
-
-Ltac by_cases_on_compress :=
-  unfold compress in *; branches; unpack; subst.
-
-(* -------------------------------------------------------------------------- *)
-
-(* Two independent steps of path compression commute. *)
-
-Lemma compress_compress:
-  forall V F (x1 z1 x2 z2 : V),
-  x1 <> x2 ->
-  compress (compress F x1 z1) x2 z2 =
-  compress (compress F x2 z2) x1 z1.
-Proof using.
-  intros. unfold compress. extens. intros.
-  split; intros; repeat (branches; unpack); subst; eauto.
-Qed.
-
-(* -------------------------------------------------------------------------- *)
-
-(* The following lemmas have weak hypotheses -- they do not rely on the
-   hypotheses of the above Section -- and this can be convenient. *)
-
-(* Path compression preserves every path whose origin [y] is not a descendant
-   of [x]. *)
-
-Lemma compress_preserves_paths_weak:
-  forall V (F : binary V) x y z r,
-  path F y r ->
-  ~ path F y x ->
-  path (compress F x z) y r.
-Proof using.
-  induction 1 using rtclosure_ind_l; intros.
-  { eauto with rtclosure. }
-  { eapply rtclosure_l.
-      { eauto using compress_preserves_other_edges, not_rtclosure_inv_neq. }
-      { eauto with rtclosure. }}
-Qed.
-
-(* Path compression preserves the representative of every vertex [y] that is
-   not a descendant of [x]. *)
-
-Lemma compress_preserves_is_repr_weak:
-  forall V (F : binary V) x y z r,
-  is_repr F y r ->
-  ~ path F y x ->
-  is_repr (compress F x z) y r.
-Proof using.
-  unfold is_repr. intros. unpack.
-  assert (r <> x). { intro. subst. tauto. }
-  eauto using compress_preserves_paths_weak, compress_preserves_roots_other_than_x.
-Qed.
-
-(* Analogous lemmas, in the reverse direction. *)
-
-Lemma compress_preserves_paths_weak_converse:
-  forall V (Fxz : binary V) x y r,
-  path Fxz y r ->
-  forall F z,
-  Fxz = compress F x z ->
-  ~ path F y x ->
-  path F y r.
-Proof using.
-  induction 1 using rtclosure_ind_l; intros; subst.
-  { eauto with rtclosure. }
-  { forwards: compress_preserves_other_edges_converse;
-      eauto using not_rtclosure_inv_neq.
-    eauto 6 with rtclosure. }
-Qed.
-
-Lemma compress_preserves_is_repr_weak_converse:
-  forall V (F : binary V) x y z r,
-  is_repr (compress F x z) y r ->
-  ~ path F y x ->
-  is_repr F y r.
-Proof using.
-  unfold is_repr. intros. unpack.
-  eauto using compress_preserves_paths_weak_converse, compress_preserves_roots_converse.
-Qed.
-
-(* -------------------------------------------------------------------------- *)
-
-(* If one wishes to reason in terms of the function [R], which maps every
-   vertex to its representative, here is how the effect of compression is
-   described. *)
-
-(* The agreement between [R] and [is_repr F] is preserved when one applies
-   [compress] to [F]. Note that [R] is unchanged, as it should be. *)
-
-Lemma compress_R_compress_agree:
-  forall V (D : set V) R F x y z,
-  is_dsf D F ->
-  fun_in_rel R (is_repr F) ->
-  F x y ->
-  path F y z ->
-  fun_in_rel
-    R
-    (is_repr (compress F x z)).
-Proof using.
-  intros. intro w.
-  erewrite <- compress_preserves_is_repr by eauto.
-  eauto.
-Qed.
-
